src/Compiler.v
@@ -1,0 +1,29 @@
+Require Core. 
+Require RTL. 
+
+Definition compile Phi t  (a : forall Var, Core.action Phi Var t) : forall Var, RTL.block Phi Var t.  
+intros. 
+apply RTL.nblock_to_block. 
+apply RTL.compile. 
+apply a. 
+Defined. 
+
+
+Lemma compile_correct (Phi : Core.state) t a :
+  let block := compile Phi t a in 
+  forall st Delta, 
+  RTL.eval_block Phi st t (block Core.eval_type) Delta =
+     Core.Sem.eval_action (a Core.eval_type) st Delta. 
+Proof. 
+  intros. 
+  rewrite <- RTL.CPS_compile_correct.        
+  rewrite <- RTL.nblock_compile_correct.
+  unfold block. unfold compile. 
+  reflexivity. 
+Qed. 
+
+Print Assumptions compile_correct. 
+
+                      
+        
+  
